TaintTracking.v
@@ -44,6 +44,9 @@ Definition join_taints t1 t2 := remove_dupes sum_eqb (t1 ++ t2).
 
 Module TaintTracking (Import ST: Semantics ListTotalMap).
 
+(* not Imported: only used for [ret_addr], and it would shadow ST's names *)
+Module MCC := MiniCETCommon(ListTotalMap).
+
 Definition tcptr := taint.
 Definition treg := ListTotalMap.t taint.
 Definition tamem := list taint.
@@ -98,7 +101,7 @@ Variant taint_ctx :=
   | CDefault.
 
 Definition taint_step (i: inst) (c: ST.cfg) (tc: tcfg) (tobs: taint) (tctx: taint_ctx) : option (tcfg * taint) :=
-  let '(pc, rs, m, s) := c in
+  let '(pc, rs, m) := c in
   let '(tpc, trs, tm, ts) := tc in
   match i with
   | <{ skip }> | <{ ctarget }> | <{ jump _ }> =>
@@ -200,11 +203,16 @@ Definition get_ctx (rs: ST.reg) (i: inst) : option taint_ctx  :=
   end.
 
 
+(* The call stack is in memory: a [ret] is final when the slot "sp" points at
+   holds no return address (see [MiniCET.ret_addr]). *)
 Definition final_cfg (p: prog) (c: ST.cfg) : bool :=
-  let '(pc, rs, m, stk) := c in
+  let '(pc, rs, m) := c in
   match ST.fetch p pc with
   | Some i => match i with
-             | IRet => if seq.nilp stk then true else false
+             | IRet => match MCC.ret_addr rs m with
+                      | Some _ => false
+                      | None => true
+                      end
              | _ => false
              end
   | None => false
@@ -213,7 +221,7 @@ Definition final_cfg (p: prog) (c: ST.cfg) : bool :=
 Definition step_taint_track (p: prog) : evaluator unit :=
   mkEvaluator _ (fun (ist : input_st) =>
     let '(c, tc, tobs) := ist in
-    let '(pc, rs, m, s) := c in
+    let '(pc, rs, m) := c in
     let '(tpc, trs, tm, ts) := tc in
     match ST.step p (S_Running c) with
     | (S_Running c', os) =>
@@ -258,7 +266,7 @@ Definition init_taint_mem (m: mem) : tamem :=
 
 Definition taint_tracking (f : nat) (p : prog) (c: cfg)
   : option (obs * list string * list nat) :=
-  let '(pc, rs, m, ts) := c in
+  let '(pc, rs, m) := c in
   let tpc := [] in
   let trs := ([], map (fun x => (x,[@inl reg_id mem_addr x])) (map_dom (snd rs))) in
   let tm := init_taint_mem m in
